wip: add VarDecl

src/Semantics/Semantics1.dfy
@@ -66,7 +66,6 @@ module Semantic {
         ensures IsDefinedOn(s1) ==> IsDefinedOn(s2)
       {  }
 
-    // TODO: make a Dafny issue (check if there already is one)
     ghost predicate Holds() {
       forall s: State :: IsDefinedOn(s.Keys) ==> s.Eval(this)
     }
@@ -152,6 +151,10 @@ module Semantic {
       case Choice(s0, s1) => s0.NoShadowing() && s1.NoShadowing()
     }
 
+    predicate WellFormed() {
+      NoShadowing() && (FVars() * BVars() == {})
+    }
+
     predicate IsDefinedOn(s: set<Variable>) {
       FVars() <= s
     }
@@ -198,6 +201,21 @@ module Semantic {
     if ss == [] then true else ss[0].NoShadowing() && SeqNoShadowing(ss[1..])
   }
 
+  predicate SeqWellFormed(ss: seq<Stmt>) {
+    // SeqNoShadowing(ss) && (SeqFVars(ss) * SeqBVars(ss) == {})
+    if ss == [] then 
+      true 
+    else 
+      && ss[0].WellFormed()
+      && (ss[0].BVars() * SeqFVars(ss[1..]) == {}) 
+      && (ss[0].BVars() * SeqBVars(ss[1..]) == {}) 
+      && SeqWellFormed(ss[1..])
+  }
+
+  lemma SeqWellFormedSeqLemma(ss: seq<Stmt>, cont: seq<Stmt>)
+    requires SeqWellFormed([Seq(ss)] + cont)
+    ensures SeqWellFormed(ss + cont)
+
   lemma SeqFunConcatLemmas(ss1: seq<Stmt>, ss2: seq<Stmt>)
     ensures SeqSize(ss1 + ss2) == SeqSize(ss1) + SeqSize(ss2)
     ensures SeqBVars(ss1 + ss2) == SeqBVars(ss1) + SeqBVars(ss2)
@@ -242,7 +260,7 @@ module Semantic {
     predicate IsFailure() {
       Error?
     }
-    function PropagateFailure<U>(f: Except<U>): Except<U>
+    function PropagateFailure<U>(): Except<U>
       requires IsFailure()
     {
       Error
@@ -252,6 +270,11 @@ module Semantic {
     {
       res
     }
+  }
+
+  function ExceptUpdate(e: Except<State>, v: Variable, b: bool): Except<State> {
+    var r :- e;
+    Ok(r.Update(v, b))
   }
 
   least predicate BigStep[nat](s: Stmt, a: State, z: Except<State>) 
@@ -267,7 +290,9 @@ module Semantic {
     case Assign(x, v) =>
       && v.IsDefinedOn(a.Keys) 
       && z == Ok(a.Update(x, a.Eval(v)))
-    case VarDecl(v, s) => exists b :: BigStep(s, a.Update(v, b), z)
+    case VarDecl(v, s) => exists b :: 
+      && BigStep(s, a.Update(v, b), ExceptUpdate(z, v, b))
+      && (z.Ok? ==> v !in z.Extract().Keys)
     case Choice(s0, s1) => BigStep(s0, a, z) || BigStep(s1, a, z)
     // case While(guard, inv, body) =>
     //   if a.Eval(guard) then
@@ -310,12 +335,8 @@ module Semantic {
             case Ok(b) => SeqBigStep(ss1[1..], b, Error)
             case _ => Error == w };
       match w
-      case Ok(st') => 
-        assert SeqBigStep([ss1[0]] + (ss1[1..] + ss2), st, Error) by {
-          assert ([ss1[0]] + (ss1[1..] + ss2))[0] == ss1[0];
-        }
-      case _ =>
-        assert BigStep(ss1[0], st, Error);
+      case Ok(st') => assert ([ss1[0]] + (ss1[1..] + ss2))[0] == ss1[0];
+      case _ => assert (ss1 + ss2)[0] == ss1[0];
     }
   }
 
@@ -336,7 +357,7 @@ module Semantic {
     }
   } 
 
-    lemma SeqBigStepChoiceLemma(s0: Stmt, s1: Stmt, cont: seq<Stmt>, st: State, out: Except<State>)
+  lemma SeqBigStepChoiceLemma(s0: Stmt, s1: Stmt, cont: seq<Stmt>, st: State, out: Except<State>)
     requires SeqBigStep([Choice(s0, s1)] + cont, st, out)
     ensures SeqBigStep([s0] + cont, st, out) || SeqBigStep([s1] + cont, st, out)
   {
@@ -350,6 +371,51 @@ module Semantic {
     } else {
       assert BigStep(s1, st, w);
       assert SeqBigStep([s1] + cont, st, out);
+    }
+  }
+
+  lemma BigStepFrameLemma(s: Stmt, v: Variable, b: Value, st: State, out: Except<State>)
+    requires BigStep(s, st, out)
+    requires v !in s.FVars()
+    requires v !in s.BVars()
+    ensures BigStep(s, st.Update(v, b), ExceptUpdate(out, v, b))
+  {
+    match s
+    case Assign(x, e) => 
+      e.EvalFVarsLemma(st, st.Update(v, b));
+      var ev := st.Eval(e);
+      assert st.Update(v, b).Update(x, ev) == st.Update(x, ev).Update(v, b);
+    case Check(e) => e.EvalFVarsLemma(st, st.Update(v, b));
+    case Assume(e) => e.EvalFVarsLemma(st, st.Update(v, b));
+    case Seq(ss) => SeqBigStepFrameLemma(ss, v, b, st, out);
+    case VarDecl(u, s) =>
+      var c :| 
+        && BigStep(s, st.Update(u, c), ExceptUpdate(out, u, c))
+        && (out.Ok? ==> u !in out.Extract().Keys);
+      BigStepFrameLemma(s, v, b, st.Update(u, c), ExceptUpdate(out, u, c));
+      assert st.Update(v, b).Update(u, c) == st.Update(u, c).Update(v, b);
+      assert ExceptUpdate(ExceptUpdate(out, u, c), v, b) == ExceptUpdate(ExceptUpdate(out, v, b), u, c) by {
+        match out
+        case Ok(st') =>
+          assert st'.Update(v, b).Update(u, c) == st'.Update(u, c).Update(v, b);
+        case _ =>
+      }
+    case Choice(s0, s1) =>
+  }
+
+  lemma SeqBigStepFrameLemma(ss: seq<Stmt>, v: Variable, b: Value, st: State, out: Except<State>)
+    requires SeqBigStep(ss, st, out)
+    requires v !in SeqFVars(ss)
+    requires v !in SeqBVars(ss)
+    ensures SeqBigStep(ss, st.Update(v, b), ExceptUpdate(out, v, b))
+  {
+    if ss == [] {
+    } else {
+      var w :| BigStep(ss[0], st, w) && match w {
+        case Ok(st') => SeqBigStep(ss[1..], st', out)
+        case _ => out == w
+      };
+      BigStepFrameLemma(ss[0], v, b, st, w);
     }
   }
 
@@ -388,17 +454,14 @@ module Semantic {
 
     function FVars(): set<Variable> 
     {
-      CtxFVars()
-      // incarnation.Values 
+      CtxFVars() + incarnation.Values
     }
 
     ghost predicate Valid() 
     {
-      && incarnation.Values <= FVars() 
-      && forall b <- bVars :: b !in incarnation.Values
+      forall b <- bVars :: b !in incarnation.Values
     }
 
-    // How to prove that `v !in incarnation.Keys` is satisfiable?
     function FreshVar(): Variable
       ensures {:axiom} FreshVar() !in incarnation.Keys
       ensures {:axiom} FreshVar() !in bVars
@@ -406,11 +469,8 @@ module Semantic {
 
 
     function AdjustState(s: State): State
-      // requires Valid()
-      // requires IsDefinedOn(s.Keys)
       requires incarnation.Values <= s.Keys
     { 
-      // IsDefinedOnConjLemma(ctx, s);
       map x: Variable | x in incarnation.Keys :: s[incarnation[x]] 
     }
 
@@ -435,18 +495,6 @@ module Semantic {
         Forall(v, Context(ctx, incarnation[v := v], bVars).Substitute(body))
     }
 
-    // function SubstituteStmt(s: Stmt): Stmt 
-    //   requires s.IsDefinedOn(incarnation.Keys)
-    //   decreases s
-    // {
-    //   match s
-    //   case Check(e) => Check(Substitute(e))
-    //   case Assume(e) => Assume(Substitute(e))
-    //   case Seq(s0, s1) => Seq(SubstituteStmt(s0), SubstituteStmt(s1))
-    //   case Assign(lhs, rhs) => Assign(incarnation[lhs], Substitute(rhs))
-    //   case VarDecl(v, s) => VarDecl(v, Context(ctx, incarnation[v:=v], bVars).SubstituteStmt(s))
-    // }
-
     function MkEntailment(e: Expr): Expr 
     {
       Implies(Conj(ctx), Substitute(e))
@@ -457,8 +505,6 @@ module Semantic {
       requires Valid()
       requires e.IsDefinedOn(incarnation.Keys)
       ensures Add(e).Valid()
-      // ensures incarnation == Add(e).incarnation
-      // ensures ctx <= Add(e).ctx
     {
       ghost var ctx' := ctx;
       var ctx := ctx + [Substitute(e)];
@@ -466,7 +512,7 @@ module Semantic {
       Context(ctx, incarnation, bVars)
     }
 
-    method AddEq(v: Variable, e: Expr) returns (vNew: Variable, context: Context)
+    method AddEq(v: Variable, e: Expr) returns (ghost vNew: Variable, context: Context)
       requires v in incarnation.Keys
       requires Valid()
       ensures context.Valid()
@@ -478,29 +524,35 @@ module Semantic {
       ensures vNew !in bVars
       ensures vNew !in FVars()
     {
-      vNew := FreshVar();
-      var ctx' := ctx + [Eq(Var(vNew), Substitute(e))];
-      FVarsEqLemma(Var(vNew), Substitute(e));
-      FVarsConjUnionLemma(ctx, [Eq(Var(vNew), Substitute(e))]);
-      var incarnation' := incarnation[v := vNew];
+      var v' := FreshVar();
+      var ctx' := ctx + [Eq(Var(v'), Substitute(e))];
+      FVarsEqLemma(Var(v'), Substitute(e));
+      FVarsConjUnionLemma(ctx, [Eq(Var(v'), Substitute(e))]);
+      var incarnation' := incarnation[v := v'];
       context := Context(ctx', incarnation', bVars);
+      vNew := v';
     }
     
     // TODO: Fix this
-    // function AddVar(v: Variable): Context
-    //   requires Valid()
-    //   ensures AddVar(v).Valid()
-    //   ensures incarnation.Keys + {v} == AddVar(v).incarnation.Keys
-    //   ensures ctx == AddVar(v).ctx
-    // {
-    //   var vNew := FreshVar();
-    //   var incarnation' := incarnation[v := vNew];
-    //   Context(ctx, incarnation', bVars)
-    // }
+    method AddVar(v: Variable) returns (ghost vNew: Variable, context: Context)
+      requires Valid()
+      ensures context.Valid()
+
+      ensures context.incarnation == incarnation[v := vNew]
+      ensures context.ctx         == ctx
+      ensures context.bVars       == bVars
+
+      ensures vNew !in incarnation.Keys
+      ensures vNew !in bVars
+      ensures vNew !in FVars()
+    {
+      var v' := FreshVar();
+      var incarnation' := incarnation[v := v'];
+      context := Context(ctx, incarnation', bVars);
+      vNew := v';
+    }
     
-    // Q: why is this not working?
     ghost predicate IsDefinedOn(s: set<Variable>) 
-      // ensures (forall e <- ctx :: e.IsDefinedOn(s))
     {
       FVars() <= s
     }
@@ -537,9 +589,7 @@ module Semantic {
 
     lemma AdjustStateSubstituteLemma'(s: State, e: Expr)
       requires forall b <- e.BVars(), x <- incarnation.Keys :: incarnation[x] == b ==> x == b
-      // requires Valid()
       requires e.IsDefinedOn(incarnation.Keys)
-      // requires IsDefinedOn(s.Keys)
       requires incarnation.Values <= s.Keys
       ensures Substitute(e).IsDefinedOn(s.Keys)
       ensures (
@@ -551,9 +601,14 @@ module Semantic {
       case Forall(v, body) => 
         var ctx' := Context(ctx, incarnation[v := v], bVars);
         SubstituteIsDefinedOnLemma(Forall(v, body)); 
-        assert forall b: bool :: AdjustState(s).Update(v, b).Eval(body) == s.Update(v, b).Eval(ctx'.Substitute(body)) by {
+        assert forall b: bool :: 
+          AdjustState(s).Update(v, b).Eval(body) == 
+          s.Update(v, b).Eval(ctx'.Substitute(body)) by 
+        {
           forall b: bool 
-            ensures AdjustState(s).Update(v, b).Eval(body) == s.Update(v, b).Eval(ctx'.Substitute(body)) {
+            ensures AdjustState(s).Update(v, b).Eval(body) == 
+              s.Update(v, b).Eval(ctx'.Substitute(body)) 
+            {
               assert AdjustState(s)[v:=b] == ctx'.AdjustState(s[v:=b]) by {
                 assert AdjustState(s)[v:=b].Keys == ctx'.AdjustState(s[v:=b]).Keys;
                 forall x: Variable {:trigger} | x in AdjustState(s)[v:=b].Keys
@@ -565,23 +620,32 @@ module Semantic {
                   }
                 }
               }
-              assert forall b <- body.BVars() {:trigger}, x <- incarnation[v:=v].Keys :: incarnation[v:=v][x] == b ==> x == b by {
+              assert forall b <- body.BVars() {:trigger}, x <- incarnation[v:=v].Keys :: 
+                incarnation[v:=v][x] == b ==> x == b by 
+              {
                 forall b <- body.BVars() {:trigger}, x <- incarnation[v:=v].Keys
                 ensures incarnation[v:=v][x] == b ==> x == b {
-                if x != v {
-                  assert e.BVars() == body.BVars() + {v};
+                  if x != v {
+                    assert e.BVars() == body.BVars() + {v};
+                  }
                 }
               }
-            }
             ctx'.AdjustStateSubstituteLemma'(s.Update(v, b), body);
           }
         }
       case Var(v) =>
       case BConst(bvalue) =>
-      case Not(ne) => assert ne.BVars() == e.BVars();
-      case And(e0, e1) => assert e0.BVars() <= e.BVars(); assert e1.BVars() <= e.BVars();
-      case Or(e0, e1) => assert e0.BVars() <= e.BVars(); assert e1.BVars() <= e.BVars();
-      case Implies(e0, e1) => assert e0.BVars() <= e.BVars(); assert e1.BVars() <= e.BVars();
+      case Not(ne) => 
+        assert ne.BVars() == e.BVars();
+      case And(e0, e1) => 
+        assert e0.BVars() <= e.BVars(); 
+        assert e1.BVars() <= e.BVars();
+      case Or(e0, e1) => 
+        assert e0.BVars() <= e.BVars(); 
+        assert e1.BVars() <= e.BVars();
+      case Implies(e0, e1) => 
+        assert e0.BVars() <= e.BVars(); 
+        assert e1.BVars() <= e.BVars();
     }
 
     lemma AdjustStateSubstituteLemma(s: State, e: Expr)
@@ -615,49 +679,6 @@ module Semantic {
     ensures (IsDefinedOnConjLemma(ctx, s); s.Eval(Conj(ctx)))
   {  }
 
-  // lemma MkEntailmentLemma(e: Expr, context: Context)
-  //   requires context.Valid()
-  //   ensures 
-  //     context.MkEntailment(e).Holds() ==> 
-  //     forall s: State :: 
-  //       context.IsSatisfiedOn(s) && context.Substitute(e).IsDefinedOn(s.Keys) ==> s.Eval(context.Substitute(e)) {
-  //     if context.MkEntailment(e).Holds() {
-  //       forall s: State | context.IsSatisfiedOn(s) && context.Substitute(e).IsDefinedOn(s.Keys)
-  //         ensures s.Eval(context.Substitute(e)) {
-  //           IsDefinedOnConjLemma(context.ctx, s);
-  //           context.FVarsSubsituteLemma(e);
-  //           assert context.MkEntailment(e).IsDefinedOn(s.Keys);
-  //           EvalConjLemma(context.ctx, s);
-  //     }
-  //   }
-  // }
-
-/*
-  []
-
-
-  x := 0
-  x := 1 
-  assume x == 1
-
-  ----
-  [x -> x']
-  x' = 0
-
-  x := 0
-  assume x == 0
-  
-*/
-
-/*
-Plan for adding: 
-    - VarDecl
-    - If 
-    - While
-*/
-
-// method VCGenAux(s: Stmt, context_in: Context, sts: set<State>, out: Except<State>) returns (result: set<Expr>, context: Context) 
-
 method VCGen(s: Stmt, context_in: Context) returns (context: Context, VCs: seq<Expr>) 
   requires s.BVars() <= context_in.bVars
   requires s.IsDefinedOn(context_in.incarnation.Keys)
@@ -682,29 +703,33 @@ method VCGen(s: Stmt, context_in: Context) returns (context: Context, VCs: seq<E
     case Check(e) =>
       VCs := [context_in.MkEntailment(e)];
       if context.MkEntailment(e).Holds() {
-        forall st: State, out: Except<State> | context.IsSatisfiedOn(st) && BigStep(Check(e), context.AdjustState(st), out) 
-           ensures out == Ok(context.AdjustState(st)) {
-            assert context.AdjustState(st).Eval(e) by { 
-              context.AdjustStateSubstituteLemma(st, e);
-              IsDefinedOnConjLemma(context.ctx, st);
-              context.SubstituteIsDefinedOnLemma(e);
-              EvalConjLemma(context.ctx, st);
-           }
+        forall st: State, out: Except<State> | 
+        context.IsSatisfiedOn(st) && BigStep(Check(e), context.AdjustState(st), out) 
+           ensures out == Ok(context.AdjustState(st)) 
+        {
+          assert context.AdjustState(st).Eval(e) by { 
+            context.AdjustStateSubstituteLemma(st, e);
+            IsDefinedOnConjLemma(context.ctx, st);
+            context.SubstituteIsDefinedOnLemma(e);
+            EvalConjLemma(context.ctx, st);
+          }
         }
       }
     case Assume(e) =>
       context := context_in.Add(e);
       VCs := [];
       FVarsConjUnionLemma(context_in.ctx, [context_in.Substitute(e)]);
-      forall st: State, out: Except<State> | context_in.IsSatisfiedOn(st) && BigStep(Assume(e), context_in.AdjustState(st), out) 
+      forall st: State, out: Except<State> | 
+        context_in.IsSatisfiedOn(st) && BigStep(Assume(e), context_in.AdjustState(st), out) 
         ensures out == Ok(context.AdjustState(st))
         ensures context.IsSatisfiedOn(st)
-        ensures context.incarnation.Values <= st.Keys {
+        ensures context.incarnation.Values <= st.Keys 
+      {
         context_in.SubstituteIsDefinedOnLemma(e);
         context_in.AdjustStateSubstituteLemma(st, e); 
       }
     case Assign(v, x) =>
-      var vNew;
+      ghost var vNew;
       vNew, context := context_in.AddEq(v, x);
       VCs := [];
       forall st: State, out: Except<State> | 
@@ -713,35 +738,40 @@ method VCGen(s: Stmt, context_in: Context) returns (context: Context, VCs: seq<E
         ensures (exists st': State :: 
             && context.incarnation.Values <= st'.Keys
             && Ok(context.AdjustState(st')) == out
-            && context.IsSatisfiedOn(st')) {
-          context_in.SubstituteIsDefinedOnLemma(x);
-          var v' := st.Eval(context_in.Substitute(x));
-          var st' := st.Update(vNew, v');
+            && context.IsSatisfiedOn(st')) 
+      {
+        context_in.SubstituteIsDefinedOnLemma(x);
+        var v' := st.Eval(context_in.Substitute(x));
+        var st' := st.Update(vNew, v');
 
-          context_in.SubstituteIsDefinedOnLemma(x);
-          FVarsEqLemma(Var(vNew), context_in.Substitute(x));
-          FVarsConjUnionLemma(context_in.ctx, [Eq(Var(vNew), context_in.Substitute(x))]);
-          
-          assert context.IsSatisfiedOn(st') by {
-            context_in.Substitute(x).EvalFVarsLemma(st, st');
-            EvalEqLemma(Var(vNew), context_in.Substitute(x), st');
-            assert forall e: Expr :: e.FVars() <= context_in.FVars() ==> st.Eval(e) ==> st'.Eval(e) by {
-              forall e: Expr | e.FVars() <= context_in.FVars() && st.Eval(e) { 
-                e.EvalFVarsLemma(st, st');
-              }
+        context_in.SubstituteIsDefinedOnLemma(x);
+        FVarsEqLemma(Var(vNew), context_in.Substitute(x));
+        FVarsConjUnionLemma(context_in.ctx, [Eq(Var(vNew), context_in.Substitute(x))]);
+        
+        assert context.IsSatisfiedOn(st') by {
+          context_in.Substitute(x).EvalFVarsLemma(st, st');
+          EvalEqLemma(Var(vNew), context_in.Substitute(x), st');
+          assert forall e: Expr :: e.FVars() <= context_in.FVars() ==> 
+            st.Eval(e) ==> st'.Eval(e) by 
+          {
+            forall e: Expr | e.FVars() <= context_in.FVars() && st.Eval(e) { 
+              e.EvalFVarsLemma(st, st');
             }
           }
-          assert context.AdjustState(st') == context_in.AdjustState(st).Update(v, context_in.AdjustState(st).Eval(x)) by {
-              context_in.AdjustStateSubstituteLemma(st, x);
-          }
         }
+        assert context.AdjustState(st') == 
+          context_in.AdjustState(st).Update(v, context_in.AdjustState(st).Eval(x)) by 
+        {
+            context_in.AdjustStateSubstituteLemma(st, x);
+        }
+      }
     case _ => assume {:axiom} false;
   }
 
 method SeqVCGen(s: seq<Stmt>, context_in: Context) returns (context: Context, VCs: seq<Expr>) 
+    requires SeqWellFormed(s)
     requires SeqBVars(s) <= context_in.bVars
     requires SeqIsDefinedOn(s, context_in.incarnation.Keys)
-    requires SeqNoShadowing(s)
 
     requires context_in.Valid()
     ensures context.Valid()
@@ -772,6 +802,7 @@ method SeqVCGen(s: seq<Stmt>, context_in: Context) returns (context: Context, VC
       match stmt 
       case Seq(ss) =>
         SeqFunConcatLemmas(ss, cont);
+        SeqWellFormedSeqLemma(ss, cont);
         context, VCs := SeqVCGen(ss + cont, context);
         if (forall e <- VCs :: e.Holds()) {
           forall st: State, out: Except<State> | context_in.IsSatisfiedOn(st) && SeqBigStep(s, context_in.AdjustState(st), out) 
@@ -797,6 +828,40 @@ method SeqVCGen(s: seq<Stmt>, context_in: Context) returns (context: Context, VC
                    || SeqBigStep([ss1] + cont, context_in.AdjustState(st), out) by
             {
               SeqBigStepChoiceLemma(ss0, ss1, cont, context_in.AdjustState(st), out);
+            }
+          }
+        }
+      case VarDecl(v, s) =>
+        ghost var vNew;
+        var context';
+        vNew, context' := context.AddVar(v);
+        context, VCs := SeqVCGen([s] + cont, context');
+        if (forall e <- VCs :: e.Holds()) { 
+          forall st: State, out: Except<State> | 
+            && context_in.IsSatisfiedOn(st)  
+            && SeqBigStep([stmt] + cont, context_in.AdjustState(st), out) 
+            ensures out.Ok?
+          { 
+            var w :| BigStep(VarDecl(v, s), context_in.AdjustState(st), w) && match w {
+              case Ok(st') => SeqBigStep(cont, st', out)
+              case _ => out == w
+            } by {
+              assert SeqBigStep([stmt] + cont, context_in.AdjustState(st), out);
+            }
+            var b :| BigStep(s, context_in.AdjustState(st).Update(v,b), ExceptUpdate(w, v, b));
+            assert context_in.AdjustState(st).Update(v,b) == context'.AdjustState(st.Update(vNew, b));
+            assert context'.IsSatisfiedOn(st.Update(vNew, b)) by {
+              forall e <- context'.ctx 
+                ensures st.Update(vNew, b).Eval(e) {
+                e.EvalFVarsLemma(st, st.Update(vNew, b));
+              }
+            }
+            assert SeqBigStep([s] + cont, context'.AdjustState(st.Update(vNew, b)), ExceptUpdate(out, v, b)) by {
+              assert BigStep(s, context'.AdjustState(st.Update(vNew, b)), ExceptUpdate(w, v, b));
+              match w 
+              case Ok(st') => 
+                SeqBigStepFrameLemma(cont, v, b, st', out);
+              case _ => 
             }
           }
         }
